\problem
%%%%%%%%%%%%%%%%%%%%%

\textcolor{Red}{\textbf{Questions:}}
Give a top-down algorithm to create Fibonacci number $n$ using memorization. The recurrence relation of the Fibonacci is:
\begin{equation}\label{eq:fibRec}
	F(n) = F(n-1) + F(n-2), F(0) = 0, F(1) = 1
\end{equation}

%%%%%%%%%%%%%%%%%%%%%
\textcolor{Green}{\textbf{Sample Solution:}}

\begin{algorithm}
	\caption{Fibonacci numbers Top down approach}\label{alg:Fib}
	Memorized-Fib(n)
	\begin{algorithmic}[1]
		\State let $F(0..n)$ be an empty array
		\For{i = 0..n}
		 \State $F(i) = -\infty$
		\EndFor
		\State Return Memorized-Fxb-Aux(n)
	\end{algorithmic}
\end{algorithm}

Algorithm \ref{alg:Fib} will return the Fibonacci number in $O(n)$ time. The helper algorithm \ref{alg:FibAux} is directly implementing the recursion relation \eqref{eq:fibRec} but instead of calculating all of the number it is using the previously memorized results from the $F(0..n)$ array.

\begin{algorithm}
	\caption{Fibonacci numbers helper algorithm}\label{alg:FibAux}
	Memorized-Fib-Aux(n)
	\begin{algorithmic}[1]
		\If{$n==0$}
		 \State Return $0$
		\ElsIf{$n==1$}
		 \State Return $1$
		\ElsIf{$n>1$ \&\& $F(n)>0 $}
		 \State Return $F(n)$
		\EndIf
		\State $F(n) = \text{Memorized-Fib-Aux}(n-1) + \text{Memorized-Fib-Aux}(n-2)$
		\State Return $F(n)$
	\end{algorithmic}
\end{algorithm}
